disk-betree/BetreeAsyncBlockCacheSystem.dfy
@@ -1,0 +1,177 @@
+include "AsyncDiskModel.dfy"
+include "PivotBetree_Refines_Betree.dfy"
+include "AsyncBlockCache.dfy"
+include "../lib/Maps.dfy"
+include "../lib/sequences.dfy"
+include "AsyncBlockCacheSystem.dfy"
+include "BetreeAsyncBlockCache.dfy"
+include "AsyncBlockCacheSystem_Refines_ThreeStateVersionedBlockInterface.dfy"
+
+module BetreeBlockCacheSystem refines AsyncDiskModel {
+  import opened Maps
+  import opened Sequences
+
+  import opened PivotBetreeSpec`Spec
+  import BC = BetreeGraphAsyncBlockCache
+  import BCS = BetreeGraphAsyncBlockCacheSystem
+  import BT = PivotBetree
+  import BTI = PivotBetreeInvAndRefinement
+  import BI = PivotBetreeBlockInterface
+  import Ref = AsyncBlockCacheSystem_Refines_ThreeStateVersionedBlockInterface
+
+  import M = BetreeAsyncBlockCache
+
+  function Ik(k: Constants) : BT.Constants
+  {
+    BT.Constants(BI.Constants())
+  }
+
+  function PersistentBetree(k: Constants, s: Variables) : BT.Variables
+  requires BCS.Inv(k, s)
+  {
+    BT.Variables(BI.Variables(Ref.PersistentGraph(k, s)))
+  }
+
+  function FrozenBetree(k: Constants, s: Variables) : BT.Variables
+  requires BCS.Inv(k, s)
+  {
+    BT.Variables(BI.Variables(Ref.FrozenGraph(k, s)))
+  }
+
+  function EphemeralBetree(k: Constants, s: Variables) : BT.Variables
+  requires BCS.Inv(k, s)
+  {
+    BT.Variables(BI.Variables(Ref.EphemeralGraph(k, s)))
+  }
+
+  predicate Init(k: Constants, s: Variables)
+  {
+    && M.Init(k.machine, s.machine)
+    && D.Init(k.disk, s.disk)
+    && BCS.Init(k, s)
+    && BT.Init(Ik(k), PersistentBetree(k, s))
+  }
+
+  predicate Inv(k: Constants, s: Variables) {
+    && BCS.Inv(k, s)
+    && BTI.Inv(Ik(k), PersistentBetree(k, s))
+    && BTI.Inv(Ik(k), FrozenBetree(k, s))
+    && BTI.Inv(Ik(k), EphemeralBetree(k, s))
+  }
+
+  // Proofs
+
+  lemma InitImpliesInv(k: Constants, s: Variables)
+    // pre and post conditions are inherited
+    //requires Init(k, s)
+    //ensures Inv(k, s)
+  {
+    BCS.InitImpliesInv(k, s);
+    BTI.InitImpliesInv(Ik(k), PersistentBetree(k, s));
+    Ref.InitImpliesGraphsEq(k, s);
+  }
+
+  /*lemma BetreeMoveStepPreservesInv(k: Constants, s: Variables, s': Variables, uiop: CrashableUIOp, step: BetreeStep)
+  requires Inv(k, s)
+  requires M.BetreeMove(k, s, s', uiop, dop, step)
+  ensures Inv(k, s')
+
+  lemma BlockCacheMoveStepPreservesInv(k: Constants, s: Variables, s': Variables, uiop: CrashableUIOp, step: BC.Step)
+  requires Inv(k, s)
+  requires M.BlockCacheMove(k, s, s', uiop, step)
+  ensures Inv(k, s')*/
+
+  /*
+    // Handles almost all cases by just showing that all graphs are
+    // equal to each other:
+    Ref.StepGraphs(k, s, s', step);
+
+    // Other cases:
+
+    if (step.machineStep.UnallocStep?) {
+      BTI.GCStepRefines(Ik(k), EphemeralBetree(k, s), EphemeralBetree(k, s'),
+          iset{step.machineStep.ref});
+    }
+
+    if (step.machineStep.TransactionStep?) {
+      BTI.
+    }
+  }
+  */
+
+  lemma BetreeMoveStepPreservesInv(k: Constants, s: Variables, s': Variables, uiop: UIOp, dop: M.DiskOp, betreeStep: BetreeStep)
+    requires Inv(k, s)
+    requires M.BetreeMove(k.machine, s.machine, s'.machine, uiop, dop, betreeStep)
+    requires D.Next(k.disk, s.disk, s'.disk, dop)
+    ensures Inv(k, s')
+  {
+    Ref.StepGraphs(k, s, s', BCS.MachineStep(dop, BC.TransactionStep(BetreeStepOps(betreeStep))));
+    assert BT.NextStep(Ik(k), EphemeralBetree(k, s), EphemeralBetree(k, s'), uiop, BT.BetreeStep(betreeStep));
+    BTI.NextPreservesInv(Ik(k), EphemeralBetree(k, s), EphemeralBetree(k, s'), uiop);
+  }
+
+  lemma BlockCacheMoveStepPreservesInv(k: Constants, s: Variables, s': Variables, uiop: UIOp, dop: M.DiskOp, step: BC.Step)
+    requires Inv(k, s)
+    requires !step.TransactionStep?
+    requires M.BlockCacheMove(k.machine, s.machine, s'.machine, uiop, dop, step)
+    requires uiop.NoOp?
+    requires D.Next(k.disk, s.disk, s'.disk, dop)
+    ensures Inv(k, s')
+  {
+    Ref.StepGraphs(k, s, s', BCS.MachineStep(dop, step));
+    if (step.UnallocStep?) {
+      //assert BI.GC(Ik(k).bck, EphemeralBetree(k, s).bcv, s'.bcv, refs)
+      assert step.ref in EphemeralBetree(k, s).bcv.view;
+      assert iset{step.ref} !! BI.LiveReferences(Ik(k).bck, EphemeralBetree(k, s).bcv);
+      assert BI.ClosedUnderPredecessor(EphemeralBetree(k, s).bcv.view, iset{step.ref});
+      assert IMapRemove1(EphemeralBetree(k, s).bcv.view, step.ref)
+          == IMapRemove(EphemeralBetree(k, s).bcv.view, iset{step.ref});
+      assert BT.GC(Ik(k), EphemeralBetree(k, s), EphemeralBetree(k, s'), uiop, iset{step.ref});
+      BTI.GCStepRefines(Ik(k), EphemeralBetree(k, s), EphemeralBetree(k, s'), uiop, iset{step.ref});
+    }
+  }
+
+  lemma CrashStepPreservesInv(k: Constants, s: Variables, s': Variables, uiop: UIOp)
+    requires Inv(k, s)
+    requires Crash(k, s, s', uiop)
+    ensures Inv(k, s')
+  {
+    Ref.StepGraphs(k, s, s', BCS.CrashStep);
+  }
+
+  lemma DiskInternalStepPreservesInv(k: Constants, s: Variables, s': Variables, uiop: UIOp, step: D.InternalStep)
+    requires Inv(k, s)
+    requires DiskInternal(k, s, s', uiop, step)
+    ensures Inv(k, s')
+  {
+    Ref.StepGraphs(k, s, s', BCS.DiskInternalStep(step));
+  }
+
+  lemma NextStepPreservesInv(k: Constants, s: Variables, s': Variables, uiop: UIOp, step: Step)
+    requires Inv(k, s)
+    requires NextStep(k, s, s', uiop, step)
+    ensures Inv(k, s')
+  {
+    match step {
+      case MachineStep(dop) => {
+        var machineStep :| M.NextStep(k.machine, s.machine, s'.machine, uiop, dop, machineStep);
+        match machineStep {
+          case BetreeMoveStep(betreeStep) => BetreeMoveStepPreservesInv(k, s, s', uiop, dop, betreeStep);
+          case BlockCacheMoveStep(blockCacheStep) => BlockCacheMoveStepPreservesInv(k, s, s', uiop, dop, blockCacheStep);
+        }
+      }
+      case DiskInternalStep(step) => DiskInternalStepPreservesInv(k, s, s', uiop, step);
+      case CrashStep => CrashStepPreservesInv(k, s, s', uiop);
+    }
+  }
+
+  lemma NextPreservesInv(k: Constants, s: Variables, s': Variables, uiop: UIOp)
+    // pre and post conditions are inherited
+    //requires Inv(k, s)
+    //requires Next(k, s, s', uiop)
+    //ensures Inv(k, s')
+  {
+    var step :| NextStep(k, s, s', uiop, step);
+    NextStepPreservesInv(k, s, s', uiop, step);
+  }
+}
